new files

Semantics.v
@@ -1,118 +1,99 @@
-Require Import ssreflect Basic SyntaxTyping List Coq.Program.Equality.
+Set Implicit Arguments.
+Unset Strict Implicit.
+Set Maximal Implicit Insertion.
+Unset Printing Implicit Defensive.
 
-(* We now define the semantics of terms according to a FullModelRaw *)
+Require Import ssreflect Basic LAF List Coq.Program.Equality.
+
+Variable LAF: LAFs.
+
 Section TermSemantics.
 
-  (* A model has four support sets: terms, primitives, positives and negatives, and a
-relation ortho between negatives and positives *)
+  (* A model structure has five basic support sets: 
+- term denotations,
+- valuations (parameterised by a QWorld),
+- label denotations, 
+- positive and negative denotations;
+Then we have
+- an orthogonality relation between negative and positive denotations;
+- a notion of semantic context
+- an interpretation for patterns
+- an interpretation for terms in a valuation in the correct QWorld
+- an interpretation for the reifeied functions 
+   *)
   
-  Record Model4PTermsRaw := {
-                      terms      : Type;
-                      primitives : Type;
-                      positives  : Type;
-                      negatives  : Type;
-                      orth: negatives*positives -> Prop
-                    }
+  Record ModelStructures := 
+    {
+      STerms   : Type;
+      Valuations : LAF.(QWorld) -> Type;
+      SLab     : Type;
+      SPos     : Type;
+      SNeg     : Type;
+      orth     : SNeg*SPos -> Prop;
+      SContexts: Contexts SLab SNeg STerms Valuations;
+      tild p   : @Dec STerms SLab SNeg (@PatDec LAF p) -> SPos;
+      SemTerms {qLab} : Valuations qLab -> Terms qLab -> STerms;
+      I {w} : SContexts w -> @Reifiable LAF w -> SNeg
+    }
   .
 
-  (* We first define semantical trees, which will interpret termtrees *)
+  Global Arguments tild {_} p _.
 
-  Definition SemTree {M} := @Tree M.(terms) M.(primitives) M.(negatives).
+  (* A useful abbreviation for semantical decompositions, which will
+  interpret term decompositions *)
 
-  (* This is a useful abbreviation for type valuations *)
+  Definition SDec {M} := @Dec M.(STerms) M.(SLab) M.(SNeg).
 
-  Definition qvaluation {M} qVar := qVar -> M.(terms).
+  (* We now suppose we have a model structure *)
 
-  (* In order to build a model of proof-terms, we require an
-interpretation of terms, 
-an interpretation of patterns, 
-and an interpretation of the reifeied functions *)
+  Variable M: ModelStructures.
 
-  Record Model4PTerms := 
-    {
-      model :> Model4PTermsRaw;
+  Definition STList := @AList LAF M.(STerms).
 
-      SemTerms {QVar}: @qvaluation model QVar -> Term QVar -> model.(terms);
-
-      SemTermsRen {QVar QVar'}:
-        forall (ren:QVar -> QVar') (sigma:@qvaluation model QVar) tau,
-          (forall xq, tau (ren xq) = sigma xq)
-          -> forall t, SemTerms sigma t = SemTerms tau (Term.(qrename) ren t);
-
-      SemTermsVar {QVar} sigma (xq:QVar): SemTerms sigma (Term.(varTerm) xq) = sigma xq;
-
-      tild : forall p:Patterns, @SemTree model (PatTree p) -> model.(positives);
-
-      I {w} : @ContType model.(terms) model.(primitives) model.(negatives) w
-              -> @Reifiable w
-              -> model.(negatives)
-    }.
-
-  Variable M: Model4PTerms.
-
-  Fixpoint SemTermList {qVar} sigma {P l} (tl:@TermList (Term qVar) P l)
-  :UTTermList M.(terms) l
+  Fixpoint SemTermList qVar sigma l (tl:TList qVar l) :STList l
     := match tl with
-        | TermNil => TermNil
-        | TermCons r so H l' tl' => TermCons (M.(SemTerms) sigma r) Logic.I (SemTermList sigma tl')
+        | TermNil => TermNil _ _
+        | TermCons so r l' tl' => TermCons so (SemTerms sigma r) (SemTermList sigma tl')
       end.
 
-  Lemma SemTermListRen {QVar QVar'}:
-        forall (ren:QVar -> QVar') (sigma:@qvaluation M QVar) tau,
-          (forall xq, tau (ren xq) = sigma xq)
-          -> forall l tl, SemTermList (l := l) sigma tl = SemTermList tau (UTTermListRen ren tl).
-  Proof.
-    intros.
-    induction l.
-    dependent inversion tl =>//.
-    dependent inversion tl =>//=.
-    rewrite (M.(SemTermsRen) (QVar := QVar) (QVar' := QVar') ren sigma tau) =>//.
-    by rewrite IHl.
-  Qed.
-
-  (* We apply our implementation of contexts to the notion of semantic
-contexts (aka valuations): positive (resp. negative) variables are
-mapped to positive (resp. negative) elements of the model *)
-  Definition SContext := @ContType M.(terms) M.(primitives) M.(negatives).
-
   (* The semantics of a negative term is a negative element of the model *)
-  Definition SemN {w} (rho:SContext w) (tm : Neg) := 
+  Definition SemN w (rho: M.(SContexts) w) (tm : Neg) := 
     match tm with
-      | rei f => M.(I) rho f
+      | rei f => I rho f
     end
   .
 
-  (* The semantics of a TermTree is a SemTree *)
-  Fixpoint SemSub {w} (rho:SContext w) {st} (v : TermTree st) {struct v} :=
-    match v in @TermTree _ s return SemTree s with
-      | tleafP xp => leafP (rho.(readp) xp)
+  (* The semantics of a TermDec is a SemTree *)
+  Fixpoint SemDec w (rho:M.(SContexts) w) {st} (v : TermDec st) {struct v} :=
+    match v in @TermDec _ _ s return SDec s with
+      | tleafP xp => leafP (readp rho xp)
       | tleafN tm => leafN (SemN rho tm)
       | tdummy    => dummy
-      | tnode s1 s2 v1 v2 => node (SemSub rho (st:=s1) v1) (SemSub rho (st:=s2) v2)
-      | tqnode s r v => qnode (M.(SemTerms) rho.(readq) r) (SemSub rho (st:=s) v)
+      | tnode s1 s2 v1 v2 => node (SemDec rho (st:=s1) v1) (SemDec rho (st:=s2) v2)
+      | tqnode s r v => qnode (SemTerms (readE rho) r) (SemDec rho (st:=s) v)
     end
   .
 
   (* The semantics of a positive term is a positive element of the model *)
-  Definition SemP {w} (rho:SContext w) (pt : Pos) := 
+  Definition SemP w (rho:M.(SContexts) w) (pt : Pos) := 
     match pt with
-        pos p v => M.(tild) p (SemSub rho v)
+        pos p v => tild p (SemDec rho v)
     end
   .
 
   (* The semantics of a command is a pair (negative element,positive
 element) of the model, that may or may not be orthogonal *) 
 
-  Definition SemC {w} (rho:SContext w) (c : Command) :=
+  Definition SemC w (rho:M.(SContexts) w) (c : Command) :=
     match c with
       | cut tm tp => (SemN rho tm,SemP rho tp) 
       | select xm tp => (rho.(readn) xm,SemP rho tp)
     end 
   .
 
-  Definition SemOptionC {w} (rho:SContext w)(oc : OptionCommand) :=
+  Definition SemOptionC w (rho:M.(SContexts) w)(oc : OptionCommand) :=
     match oc with
-      | some c => Some(SemC (rho:SContext w) c)
+      | some c => Some(SemC (rho:M.(SContexts) w) c)
       | none => None
     end
   .
@@ -121,9 +102,10 @@ End TermSemantics.
 
 
 
+Section TypeSemantics.
 
-(************************************************************************)
-(* We now want to define the semantical interpretation of types/formulae.
+  (************************************************************************)
+  (* We now want to define the semantical interpretation of types/formulae.
 
 This is traditionally done "by induction on types/formulae".
 In our setting, we do not have an inductive structure for types/formulae;
@@ -142,100 +124,105 @@ have to be SMALLER than the decomposed molecule.
 
 We formalise this. *)
 
-(* A molecule belongs to a TypeTree, as if it were a set *)
+  (* A molecule belongs to a TypeTree, as if it were a set *)
 
-Inductive  belong {l}
-: forall l' st, TypeTree st l' -> Molecule l -> Prop
-  :=
-  | rel_leaf  : forall B, belong l sleafN (TleafN B) B
-  | rel_node1 : forall B l' s1 s2 t1 t2,
-                  belong l' s1 t1 B -> belong l' (snode s1 s2) (Tnode t1 t2) B
-  | rel_node2 : forall B l' s1 s2 t1 t2,  
-                  belong l' s2 t2 B -> belong l' (snode s1 s2) (Tnode t1 t2) B
-  | rel_nodeq : forall so B l' s t, 
-                  belong (so::l') s t B
-                  -> belong l' (sqnode s) (Tqnode so t) B
-.
+  Inductive  belong l
+  : forall l' st, TypingDec (QST := LAF) st l' -> @Molecule LAF l -> Prop
+    :=
+    | rel_leaf  : forall B, belong (TleafN B) B
+    | rel_node1 : forall B l' s1 s2 (t1:TypingDec s1 l') (t2:TypingDec s2 l'),
+                    belong t1 B -> belong (Tnode t1 t2) B
+    | rel_node2 : forall B l' s1 s2 (t1:TypingDec s1 l') (t2:TypingDec s2 l'),  
+                    belong t2 B -> belong (Tnode t1 t2) B
+    | rel_nodeq : forall so B l' s (t:TypingDec s (so::l')), 
+                    belong t B
+                    -> belong (Tqnode t) B
+  .
 
-Inductive relation : DPair Molecule -> DPair Molecule -> Prop :=
-  relation_base:
-    forall p l l' Delta A B, PatternsTyped p Delta A
-               -> belong l' (PatTree p) Delta B
-               -> relation (existS _ l B) (existS _ l' A).
+  Inductive relation : DPair (@Molecule LAF) -> DPair (@Molecule LAF) -> Prop :=
+    relation_base:
+      forall p l l' Delta A B, PatternsTyped p Delta A
+                      -> belong Delta B
+                      -> relation (existS _ l B) (existS _ l' A).
 
-Hypothesis welf: well_founded relation.
+  Global Arguments relation_base p {l l'} Delta A B _ _.
 
+  (****************************************************************)
+  (* We now define the semantics of types according to a ModelRaw *)
 
-(****************************************************************)
-(* We now define the semantics of types according to a ModelRaw *)
-
-Section TypeSemantics.
-
-  Definition Pard {A B} {M:Model4PTerms} 
-             (f: forall a:DPair A, UTTermList (terms M) (ex1 a) -> B)
-             {qVar} sigma a
-    := f {{ ex1 a, getA (qVar := qVar) a }} (SemTermList M sigma (getTerms a)).
+  Definition Pard {A B M} 
+             (f: forall a:DPair A, STList M (ex1 a) -> B)
+             {qLab} sigma a
+    := f {{ ex1 a, getA (qLab := qLab) a }} (SemTermList sigma (getTerms a)).
   
-  Record ModelRaw :=
-    { model4PTerms :> Model4PTerms;
-      sortsI: Sorts -> model4PTerms.(terms) -> Prop;
-      sortscompat {qVar}: forall Sigma sigma,
-                            (forall qvar:qVar, sortsI (Sigma qvar) (sigma qvar))
-                            -> forall s t, 
-                                SortingRel Sigma t s
-                                -> sortsI s (model4PTerms.(SemTerms) sigma t);
+  Record RealisabilityAlg :=
+    { modelStructure :> ModelStructures;
+      welf: well_founded relation;
+      SemSorts : Sorts LAF -> modelStructure.(STerms) -> Prop;
+      SemSoCont qLab: SoContexts qLab -> modelStructure.(Valuations) qLab -> Prop;
+      SemSoCompat qLab: forall Sigma r s sigma, 
+                            SortingRel (qLab := qLab) Sigma r s
+                            -> SemSoCont Sigma sigma
+                            -> SemSorts s (SemTerms sigma r);
 
-      atomI : forall a:DPair Atom,
-                UTTermList model4PTerms.(terms) (ex1 a)
-                -> model4PTerms.(primitives) -> Prop;
+      SemAtom : forall a:DPair Atom,
+                STList modelStructure (ex1 a)
+                -> modelStructure.(SLab) -> Prop;
 
-      atomI_eq {qVar sigma}: forall a b p, is_eq a b
-                                  -> Pard (qVar := qVar) atomI sigma a p -> Pard atomI sigma b p
+      SemAtom_eq qLab sigma: 
+        forall a b p, is_eq a b
+                 -> Pard (qLab := qLab) (@SemAtom) sigma a p -> Pard (@SemAtom) sigma b p
 
     }.
 
-  Variable M: ModelRaw.
+  Global Arguments SemAtom {_} a _ _.
+
+  (* We now assume we have a realisability algebra *)
+
+  Variable M: RealisabilityAlg.
 
   (* Here is the orthogonal of a set of positive elements of the model, or more precisely a predicate P: M.(positive) -> Prop *)
-  Definition ortho P :=
-    fun tm => forall tp: M.(positives), P tp -> M.(orth) (tm,tp).
+  Definition ortho P tm :=
+    forall tp: M.(SPos), P tp -> orth (tm,tp).
 
   (* Given a molecule A, this is a predicate on positives, that holds if
 this positive is of the form (M.(tild) p v), for some pattern p and
-some SemTree v such that p decomposes A into some TypeTree Delta and v is
+some SDec v such that p decomposes A into some TypeTree Delta and v is
 in the semantics of Delta. The semantics of TypeTrees not being defined
 yet, it is passed as an argument SemContext.  *)
 
+  Unset Implicit Arguments.
+
   Inductive PV
             (A: DPair Molecule)
-            (SemContext: forall st, TypeTree st (ex1 A)
-                               -> forall tl:UTTermList M.(terms) (ex1 A), SemTree st -> Prop)
-            (tl: UTTermList M.(terms) (ex1 A))
-  : M.(positives) -> Prop :=
+            (SemTDec: forall st, TypingDec st (ex1 A)
+                               -> forall tl:STList M (ex1 A), SDec st -> Prop)
+            (tl: STList M (ex1 A))
+  : M.(SPos) -> Prop :=
     pv : forall p Delta v,
            PatternsTyped p Delta (ex2 A)
-           -> SemContext (PatTree p) Delta tl v 
-           -> PV A SemContext tl (M.(tild) p v).
+           -> SemTDec (PatDec p) Delta tl v 
+           -> PV A SemTDec tl (tild p v).
 
-  (* The interpretation (predicate on SemTrees) of a TypeTree Delta, given
+  (* The interpretation (predicate on SDecs) of a TypeTree Delta, given
 a valuation sigma and a function f that provides the negative
 interpretation of any molecule B in Delta *)
 
-  Definition SemCont_aux
-             (f : forall (A:DPair Molecule), UTTermList M.(terms) (ex1 A) -> M.(negatives) -> Prop)
+  Definition SemTDec_aux
+             (f : forall (A:DPair (@Molecule LAF)), STList M (ex1 A) -> M.(SNeg) -> Prop)
              l
              st
-             (Delta : TypeTree st l)
-             (tl:UTTermList M.(terms) l)
-             (v: @SemTree M st)
+             (Delta : TypingDec (QST := LAF) st l)
+             (tl:STList M l)
+             (v: @SDec M st)
   : Prop.
     move : l tl Delta.
     induction st => l tl Delta; inversion Delta; inversion v.
-    exact (M.(atomI) {{ l, X }} tl X0).
+    exact (SemAtom {{ l, X }} tl X0).
     exact (f {{ l, X }} tl X0).
     exact True.
     exact (IHst1 X1 l tl X /\ IHst2 X2 l tl X0).
-    exact ( M.(sortsI) so X0 /\ IHst X1 (so::l) (TermCons X0 (Logic.I) tl) X).
+    exact (SemSorts so X0 /\ IHst X1 (so::l) (TermCons so X0 tl) X).
   Defined.
 
 
@@ -246,14 +233,14 @@ positive interpretation of any molecule B smaller than A *)
 
   Definition SemPos_aux
              (A: DPair Molecule)
-             (f : forall B, relation B A -> UTTermList M.(terms) (ex1 B) -> M.(positives) -> Prop)
-    := PV A (SemCont_aux (fun B tl tm => exists h:relation B A, ortho (f B h tl) tm) (ex1 A)).
+             (f : forall B, relation B A -> STList M (ex1 B) -> M.(SPos) -> Prop)
+    := PV A (SemTDec_aux (fun B tl tm => exists h:relation B A, ortho (f B h tl) tm) (ex1 A)).
 
   (* The positive interpretation (predicate on positives) of a molecule
 A, given a type valuation sigma. Fixpoint of the previous function, built on
 the well-founded relation on molecules. *)
 
-  Definition SemPos := Fix welf _ (SemPos_aux).
+  Definition SemPos := Fix M.(welf) _ (SemPos_aux).
 
   (* The negative interpretation (predicate on negatives) of a molecule
 A, given a valuation sigma. It is built as the orthogonal of the positive
@@ -261,12 +248,12 @@ interpretation of A.  *)
 
   Definition SemNeg A tl := ortho (SemPos A tl).
 
-  (* A new version of the interpretation (predicate on SemTrees) of a
+  (* A new version of the interpretation (predicate on SDecs) of a
 TypeTree Delta, given a valuation sigma, but this time the predicate
 used as the negative interpretation of any molecule B in Delta is not
 passed as a parameter, it is the actual interpretation SemNeg *)
 
-  Definition SemCont {l st} := SemCont_aux SemNeg l st.
+  Definition SemTDec {l st} := SemTDec_aux (@SemNeg) l st.
 
   (* The definition of SemPos is so far quite cryptic, because of the
 induction that was necessary for the definition to be sound. The
@@ -276,16 +263,16 @@ before that we need the following two lemmas. *)
   Lemma F_ext_aux:
     forall (x:DPair Molecule)
       (f g: forall y:DPair Molecule, 
-              relation y x -> UTTermList M.(terms) (ex1 y) -> M.(positives) -> Prop),
+              relation y x -> STList M (ex1 y) -> M.(SPos) -> Prop),
       (forall (y:DPair Molecule) (p:relation y x) tl d, f y p tl d <-> g y p tl d) 
-      -> forall st l (Delta:TypeTree st l),
-          forall tl' (v : SemTree st),
-            SemCont_aux (fun (B : DPair Molecule) tl (tm : negatives M) =>
+      -> forall st l (Delta:TypingDec st l),
+          forall tl' (v : SDec st),
+            SemTDec_aux (fun (B : DPair Molecule) tl (tm : M.(SNeg)) =>
                            exists h : relation B x, ortho (f B h tl) tm)
-                        l st Delta tl' v ->
-            SemCont_aux (fun (B : DPair Molecule) tl (tm : negatives M) =>
+                        _ _ Delta tl' v ->
+            SemTDec_aux (fun (B : DPair Molecule) tl (tm : M.(SNeg)) =>
                            exists h : relation B x, ortho (g B h tl) tm)
-                        l st Delta tl' v .
+                        _ _ Delta tl' v .
   Proof.
     move => A f g H st.
 
@@ -296,7 +283,7 @@ before that we need the following two lemmas. *)
     unfold ortho.
     elim => h H1.
     exists h.
-    move => tp H2.
+    move => // tp H2.
     apply: H1.
     by apply H.
 
@@ -312,7 +299,7 @@ before that we need the following two lemmas. *)
   Lemma F_ext :
     forall (x:DPair Molecule)
       (f g: forall y:DPair Molecule, 
-              relation y x -> UTTermList M.(terms) (ex1 y) -> M.(positives) -> Prop),
+              relation y x -> STList M (ex1 y) -> M.(SPos) -> Prop),
       (forall (y:DPair Molecule) (p:relation y x) tl d, f y p tl d <-> g y p tl d) 
       -> forall tl d, SemPos_aux x f tl d -> SemPos_aux x g tl d.
   Proof.
@@ -327,24 +314,24 @@ before that we need the following two lemmas. *)
 
   Lemma Fix_F_inv :
     forall (x:DPair Molecule) tl d (r s:Acc relation x),
-      Fix_F (fun A => UTTermList (terms M) (ex1 A) -> M.(positives) -> Prop) 
+      Fix_F (fun A => STList M (ex1 A) -> M.(SPos) -> Prop) 
             SemPos_aux r tl d 
       <-> 
-      Fix_F (fun A => UTTermList (terms M) (ex1 A) -> M.(positives) -> Prop)
+      Fix_F (fun A => STList M (ex1 A) -> M.(SPos) -> Prop)
             SemPos_aux s tl d.
   Proof.
-    move => A; induction (welf A).
+    move => A; induction (M.(welf) A).
     move => tl d r s.
     rewrite <- (Fix_F_eq _ _ r). 
     rewrite <- (Fix_F_eq _ _ s).
     split.
-    apply (F_ext _
+    apply (@F_ext _ 
                  (fun (y : DPair Molecule) (p : relation y x)  =>
-                    Fix_F _ SemPos_aux (Acc_inv r p))) => //=.
+                    Fix_F _ (@SemPos_aux) (Acc_inv r p))) => //=.
     auto.
-    apply (F_ext _
+    apply (@F_ext _
                  (fun (y : DPair Molecule) (p : relation y x)  =>
-                    Fix_F _ SemPos_aux (Acc_inv s p))) => //=.
+                    Fix_F _ (@SemPos_aux) (Acc_inv s p))) => //=.
     auto.
   Qed.
 
@@ -356,7 +343,7 @@ but with the actual SemPos taking the place of the parameter f *)
     forall A tl tp, 
       SemPos A tl tp 
       <-> PV A 
-           (SemCont_aux (fun B tl' tm => exists h:relation B A, ortho (SemPos B tl') tm) (ex1 A))
+           (SemTDec_aux (fun B tl' tm => exists h:relation B A, ortho (SemPos B tl') tm) (ex1 A))
            tl
            tp.
   Proof.
@@ -367,16 +354,16 @@ but with the actual SemPos taking the place of the parameter f *)
 
   (* Characterisation of SemPos: The second step is to have a
 reformulation which drops the requirement B smaller than A in its use
-of SemCont_aux (that requirement was needed for the well-foundedness
+of SemTDec_aux (that requirement was needed for the well-foundedness
 of the definition of SemPos) *)
 
-  Lemma SemPosCont_aux1 : 
-    forall A st l (Delta:TypeTree st l) tl (v:SemTree st), 
-      (forall B : DPair Molecule, belong l st Delta (ex2 B) -> relation B A)
-      -> SemCont_aux (fun (B : DPair Molecule) tl' (tm : negatives M) => 
+  Lemma SemPosDec_aux1 : 
+    forall A st l (Delta:TypingDec st l) tl (v:SDec st), 
+      (forall B : DPair Molecule, belong Delta (ex2 B) -> relation B A)
+      -> SemTDec_aux (fun (B : DPair Molecule) tl' (tm : M.(SNeg)) => 
                        ortho (SemPos B tl') tm) 
                     l st Delta tl v      
-      -> SemCont_aux (fun (B : DPair Molecule) tl' (tm : negatives M) =>
+      -> SemTDec_aux (fun (B : DPair Molecule) tl' (tm : M.(SNeg)) =>
                        exists _ : relation B A, ortho (SemPos B tl') tm)
                     l st Delta tl v.
   Proof.
@@ -386,7 +373,7 @@ of the definition of SemPos) *)
       dependent induction v => H //; simpl.
 
       + move => H1.
-        assert (belong _ sleafN (TleafN m) m).
+        assert (belong (TleafN m) m).
         apply rel_leaf.
         assert (relation (existS _ l m) A).
         apply H => //=.
@@ -411,12 +398,12 @@ of the definition of SemPos) *)
         apply: rel_nodeq => //.
     Qed.
 
-  Lemma SemPosCont_aux2: 
-    forall A st l (Delta:TypeTree st l) tl (v:SemTree st), 
-      SemCont_aux (fun (B : DPair Molecule) tl' (tm : negatives M) =>
+  Lemma SemPosDec_aux2: 
+    forall A st l (Delta:TypingDec st l) tl (v:SDec st), 
+      SemTDec_aux (fun (B : DPair Molecule) tl' (tm : M.(SNeg)) =>
                        exists _ : relation B A, ortho (SemPos B tl') tm)
                     l st Delta tl v
-      -> SemCont_aux (fun (B : DPair Molecule) tl' (tm : negatives M) =>
+      -> SemTDec_aux (fun (B : DPair Molecule) tl' (tm : M.(SNeg)) =>
                        ortho (SemPos B tl') tm) 
                     l st Delta tl v.
   Proof.
@@ -429,14 +416,14 @@ of the definition of SemPos) *)
     + by move => [H4 H]; split => //; apply: IHst.
     Qed.
 
-  Lemma SemPosCont_aux: 
+  Lemma SemPosDec_aux: 
     forall A tl tp, 
       PV A 
-         (SemCont_aux (fun B tl' tm => ortho (SemPos B tl') tm) (ex1 A))
+         (SemTDec_aux (fun B tl' tm => ortho (SemPos B tl') tm) (ex1 A))
          tl
          tp      
       <-> PV A 
-           (SemCont_aux (fun B tl' tm => exists h:relation B A, ortho (SemPos B tl') tm) (ex1 A))
+           (SemTDec_aux (fun B tl' tm => exists h:relation B A, ortho (SemPos B tl') tm) (ex1 A))
            tl
            tp.
   Proof.
@@ -444,12 +431,12 @@ of the definition of SemPos) *)
     intros.
     split => H;elim H;clear H;intros; apply (pv {{ lA,Araw }} _ tl p Delta v) => //=.
     + assert  (forall (B : DPair Molecule),
-                 belong lA (PatTree p) Delta (ex2 B) -> relation B {{ lA,Araw }}).
+                 belong Delta (ex2 B) -> relation B {{ lA,Araw }}).
         * elim => lB Braw.
           intros.
-          apply (relation_base p lB lA Delta) => //=.
-      apply SemPosCont_aux1 =>//.
-      apply (SemPosCont_aux2 {{ lA,Araw }}) =>//.
+          apply (relation_base p Delta) => //=.
+      apply SemPosDec_aux1 =>//.
+      apply (SemPosDec_aux2 {{ lA,Araw }}) =>//.
   Qed.
 
 
@@ -458,19 +445,33 @@ definition we would actually like, and notice that, when unfolded, it
 is equivalent to the actual definition by using the previous two
 lemmas *)
 
-  Theorem SemPosCont : forall A tl tp, SemPos A tl tp <-> PV A (@SemCont (ex1 A)) tl tp.
+  Theorem SemPosDec : forall A tl tp, SemPos A tl tp <-> PV A (@SemTDec (ex1 A)) tl tp.
   Proof.
     intros;split; intro.
-    apply SemPosCont_aux;apply SemPos_Fix => //=.
-    apply SemPos_Fix;apply SemPosCont_aux => //=.
+    apply SemPosDec_aux;apply SemPos_Fix => //=.
+    apply SemPos_Fix;apply SemPosDec_aux => //=.
   Qed.
+
+  (* We define the interpretation of a typing context as a predicate on
+semantic contexts *)
+
+  Definition SemCont {w}: TContext w -> M.(SContexts) w -> Prop
+    := fun Gamma rho =>
+      SemSoCont (TreadE Gamma) (readE rho)
+      /\ (forall xp, (Pard SemAtom (readE rho)) (Treadp Gamma xp) (readp rho xp))
+      /\ (forall xn, (Pard SemNeg (readE rho)) (Treadn Gamma xn) (readn rho xn)).
 
 End TypeSemantics.
 
+Arguments SemAtom {_} _ _ _.
 Arguments SemPos {M} _ _ _.
-Arguments SemCont {M} {l st} _ _ _.
+Arguments SemTDec {M l st} _ _ _.
 Arguments SemNeg {M} _ _ _.
-Arguments atomI {m} _ _ _.
+Arguments SemCont {M w} _ _.
+
+Set Implicit Arguments.
+Unset Strict Implicit.
+Set Maximal Implicit Insertion.
 
 (**************************************)
 
@@ -482,166 +483,101 @@ orthogonality relation be closed "under anti-reduction" *)
 
   Record FullModel := 
     {
-      M0 :> ModelRaw;
+      M0 :> RealisabilityAlg;
 
-      treevalue {st}: @SemTree M0 st -> Prop;
+      TypingCorr w st :
+        forall (rho:M0.(SContexts) w) Gamma l (Delta:TypingDec st l) tl v, 
+          SemCont Gamma rho
+          -> SemTDec Delta (SemTermList (readE rho) tl) v
+          -> SemCont (Textends [Delta,tl] Gamma) (extends v rho);
 
-      stab {w} :
-        forall (f: Reifiable) (rho: SContext M0 w) (p: Patterns) (v: SemTree (PatTree p)) c,
-          treevalue v
-          -> f p =cis= c
-          -> M0.(orth) (SemC M0 (Context.(extends) v rho) c)
-          -> M0.(orth) (M0.(I) rho f, M0.(tild) p v)
+      Stability w :
+        forall (f: Reifiable w) (rho: M0.(SContexts) w) (p: Patterns LAF)
+          l Delta (tl:STList M0 l) (v: SDec (PatDec p)) c,
+          f p =cis= c
+          -> SemTDec Delta tl v
+          -> orth (SemC (extends v rho) c)
+          -> orth (I rho f, tild p v)
     }.
-
-  Variable M:FullModel.
-
-  (* We define the interpretation of a typing context as a predicate on
-semantic contexts *)
-
-  Definition compat {w w'} val: @ContType Sorts 
-                                  (Par Atom w'.(QVar))
-                                  (Par Molecule w'.(QVar))
-                                  w
-                             -> SContext M w -> Prop
-    := Contlift (w := w) M.(sortsI)(Pard atomI val) (Pard SemNeg val).
-
-  Lemma SemPos2Treelift  qVar qVar' (sigma:qvaluation qVar) (tau:qvaluation qVar') (ren:qVar -> qVar') st qnew l Delta (tl:UTTermList M.(terms) l) tl' v 
-  :  (forall xq, tau (ren xq) = sigma xq)
-     -> correctNaming tau v qnew
-     -> tl = SemTermList M tau tl'
-     -> SemCont (M := M)(st := st) Delta tl v
-     -> Treelift M.(sortsI) (Pard atomI tau) (Pard SemNeg tau) (namedTypeTree tl' Delta qnew) v.
-
-  Proof.
-    move : l Delta tl tl'.
-    induction st => l Delta tl tl' H0 H1  H2; dependent induction v =>//=; dependent induction Delta =>//=; dependent induction qnew =>//=.
-    rewrite /getA/getTerms/ex2. 
-    by rewrite H2.
-    rewrite /getA/getTerms/ex2. 
-    by rewrite H2.
-    simpl in H1. 
-    elim: H1 => H3 H4.
-    move => [I1 I2]; split ; [apply (IHst1 _ _ _ _ tl) | apply (IHst2 _ _ _ _ tl) ] =>//.
-    simpl in H1. 
-    elim: H1 => H3 H4.
-    elim => H5 H6; split => //.
-    clear IHv IHDelta IHqnew.
-    apply (IHst _ _ _ _ (TermCons c Logic.I tl)) =>//.
-    simpl.
-    by rewrite SemTermsVar H3 H2.
-Qed.
-
-  Lemma compatrename w w' Gamma rho sigma tau (ren:w.(QVar) -> w'.(QVar))
-  (pi: forall xq, tau (ren xq) = sigma xq)
-  : compat sigma Gamma rho -> compat tau (Contmap (w:=w) (fun i => i) (ParRen ren) (ParRen ren) Gamma) rho.
-  Proof.
-    rewrite/compat/Contlift/Contmap;elim => H1 [H2 H3] /=.
-                                              split => //;split.
-    move => xp.
-    move: (H2 xp); clear H2 H3.
-    elim : (readp Gamma xp) => l [a tl]. 
-    rewrite /Pard/ParRen/ex1/getA/getTerms/ex2; simpl.
-    rewrite (SemTermListRen (QVar := w.(QVar)) (QVar' := w'.(QVar)) M ren sigma tau) =>//.
-    move => xn.
-    move: (H3 xn); clear H2 H3.
-    elim : (readn Gamma xn) => l [a tl]. 
-    rewrite /Pard/ParRen/ex1/getA/getTerms/ex2; simpl.
-    rewrite (SemTermListRen (QVar := w.(QVar)) (QVar' := w'.(QVar)) M ren sigma tau) =>//.
-Qed.
 
   (* Here is finally the Adequacy Lemma *)
 
-  Hypothesis HValues: forall st (v:SemTree st) l Delta tl, SemCont (l := l) Delta tl v -> treevalue M v.
-
-  Theorem adequacy:
-    forall (w:World) (Gamma:TContext w),
+  Theorem adequacy (M:FullModel) :
+    forall (w:World LAF) (Gamma:TContext w),
       (forall pt A,
-         TypingPos Gamma pt A
-         ->  forall rho, compat rho.(readq) Gamma rho
-                 -> Pard SemPos rho.(readq) A (SemP M rho pt)
+         PosTyping Gamma pt A
+         ->  forall rho:M.(SContexts) w, SemCont Gamma rho
+                 -> Pard SemPos (readE rho) A (SemP rho pt)
       )
-      /\ (forall l st (v:TermTree st) Delta tl,
-           TypingSub Gamma v Delta tl
-           ->  forall rho, compat rho.(readq) Gamma rho
-                   -> SemCont (l:=l) Delta (SemTermList M rho.(readq) tl) (SemSub M rho v)
+      /\ (forall l st (v:TermDec st) Delta tl,
+           DecTyping Gamma v Delta tl
+           ->  forall rho:M.(SContexts) w, SemCont Gamma rho
+                   -> SemTDec (l:=l) Delta (SemTermList (readE rho) tl) (SemDec rho v)
         )
       /\ (forall nt A,
-           TypingNeg Gamma nt A
-           ->  forall rho, compat rho.(readq) Gamma rho
-                   -> Pard SemNeg rho.(readq) A (SemN M rho nt)
+           NegTyping Gamma nt A
+           ->  forall rho:M.(SContexts) w, SemCont Gamma rho
+                   -> Pard SemNeg (readE rho) A (SemN rho nt)
         )
       /\ (forall c,
-           TypingOptionCommand Gamma c
-           ->  forall rho, compat rho.(readq) Gamma rho
-                   -> exists csem, (SemOptionC M rho c) = Some csem /\ M.(orth) csem)
+           OptionCommandTyping Gamma c
+           ->  forall rho:M.(SContexts) w, SemCont Gamma rho
+                   -> exists csem, (SemOptionC rho c) = Some csem /\ orth csem)
       /\ (forall c,
-           TypingCommand Gamma c
-           ->  forall rho, compat rho.(readq) Gamma rho
-                   -> M.(orth) (SemC M rho c))
+           CommandTyping Gamma c
+           ->  forall rho:M.(SContexts) w, SemCont Gamma rho
+                   -> orth (SemC rho c))
   .
+  Proof.
+
     apply typing_ind;intros;
     [
       (* Typing a positive *)
-      apply SemPosCont; by apply (pv _ {{l, A}} _ _ p Delta) =>//; apply (H rho H0)
+      apply SemPosDec; by apply (pv _ {{l, A}} _ _ p Delta) =>//; apply (H rho H0)
 
       (* Typing a positive leaf of Sub *)
-      | unfold SemCont => //=;
-        by apply (M.(atomI_eq) (qVar:= w.(QVar)) (sigma:= rho.(readq)) 
-                        (Gamma.(readp) xp) {{l, (x, tl)}}) => //;
-        elim: H => _ [H _]; apply:H 
+      | unfold SemTDec => //= ;
+        by apply (SemAtom_eq i) => //;
+        elim: H => _ [H _]; apply:H
 
       (* Typing a negative leaf of Sub *)
-      | unfold SemCont => //= ; by apply H
+      | unfold SemTDec => //= ; by apply H
 
       (* Typing a dummy leaf of Sub *)
-      | unfold SemCont => //= 
+      | unfold SemTDec => //= 
 
       (* Typing a node of Sub *)
-      | by unfold SemCont => //=; unfold SemCont in H, H0; split; [apply H|apply H0]
+      | by unfold SemTDec => //=; unfold SemTDec in H, H0; split; [apply H|apply H0]
 
       (* Typing a qnode of Sub *)
-      | unfold SemCont => //=; 
+      | unfold SemTDec => //=; 
         by split;
-           [ apply (sortscompat M (Gamma.(readq))); move:H0;rewrite/compat/Contlift;elim => H2 _ 
+           [ apply (SemSoCompat (Sigma:=TreadE Gamma)); move:H0;rewrite/SemCont;elim => H2 _ 
            | apply H ]
 
       (* Typing a negative *)
       | 
 
       (* Typing an optional command *)
-      | by exists (SemC M rho c); split; [| apply: H]
+      | by exists (SemC rho c); split; [| apply: H]
 
       (* Typing a cut *)
-      | by rewrite /SemCont/Pard/SemNeg/ortho/getA/getTerms in H;apply H =>//; apply H0
+      | by rewrite /SemTDec/Pard/SemNeg/ortho/getA/getTerms in H;apply H =>//; apply H0
 
       (* Typing a select *)
-      | by rewrite /SemC/compat/Pard/SemNeg/ortho in H0;apply H0;apply H
+      | by rewrite /SemC/SemCont/Pard/SemNeg/ortho in H0;apply H0;apply H
     ].
-    
+
     (* Typing a negative *)
     rewrite /Pard/SemNeg/ortho/getA/getTerms => /= tp H1.
-    assert (PV M {{ l,A }} (@SemCont M l) (SemTermList M (readq rho) tl) tp)
-      by apply SemPosCont =>//=.
+    assert (PV M {{ l,A }} (@SemTDec M l) (SemTermList (readE rho) tl) tp)
+      by apply SemPosDec =>//=.
     elim H2 => /= p Delta v H3 H4; clear H2.
-    have H6: (exists csem : negatives M * positives M,
-                SemOptionC (w:=Context.(wextends) (PatTree p) w)
-                           M
-                           (Context.(extends) v rho)
-                           (f p) = Some csem
-                /\ orth M csem).
+    have H6: (exists csem : SNeg M * SPos M,
+                SemOptionC (extends v rho) (f p) = Some csem
+                /\ orth csem).
     apply: (H p Delta) => //.
-    apply (Context.(corr) (w:=w) (st:=PatTree p)).
-    apply (SemPos2Treelift _ _ rho.(readq) _ (qinject Context (PatTree p) w) (PatTree p) (qnew Context (PatTree p) w) l Delta (SemTermList M rho.(readq) tl) (UTTermListRen (qinject Context (PatTree p) w) tl))=> // .
-    move => xq.
-    apply (Context.(extends_qinject) (w:=w) (st:=PatTree p)).
-    apply (Context.(extends_qnew) (w:=w) (st:=PatTree p)).
-    apply SemTermListRen.
-    move => xq.
-    apply (Context.(extends_qinject) (w:=w) (st:=PatTree p)).
-    apply (compatrename _ _ _ _ rho.(readq)) => //.
-    move => xq.
-    apply (Context.(extends_qinject) (w:=w) (st:=PatTree p)).
+    apply: TypingCorr => //.
     elim: H6 => csem [H7 H8].
     have : exists c, (f p = some c).
     move : H7.
@@ -649,8 +585,7 @@ Qed.
     by move => c _; exists c.
     move => H9;discriminate H9.
     elim => c H9.
-    apply (M.(stab) (w:=w) _ _ _ _ c).
-    apply (HValues _ _ _ _ _ H4) =>//.
+    apply (Stability (Delta := Delta) (tl := (SemTermList (readE rho) tl)) (c := c)) => //.
     by rewrite H9.
     move:H7.
     rewrite H9 => /= H7; injection H7; clear H7 => H7; rewrite H7 =>//.
@@ -659,3 +594,72 @@ Qed.
 End Adequacy.
 
 Print Assumptions adequacy.
+
+(* Lemma SemTermListRen {QVar QVar'}: *)
+(*       forall (ren:QVar -> QVar') (sigma:@qvaluation M QVar) tau, *)
+(*         (forall xq, tau (ren xq) = sigma xq) *)
+(*         -> forall l tl, SemTermList (l := l) sigma tl = SemTermList tau (UTTermListRen ren tl). *)
+(* Proof. *)
+(*   intros. *)
+(*   induction l. *)
+(*   dependent inversion tl =>//. *)
+(*   dependent inversion tl =>//=. *)
+(*   rewrite (M.(SemTermsRen) (QVar := QVar) (QVar' := QVar') ren sigma tau) =>//. *)
+(*   by rewrite IHl. *)
+(* Qed. *)
+
+
+(*   Lemma SemPos2Treelift  qVar qVar' (sigma:qvaluation qVar) (tau:qvaluation qVar') (ren:qVar -> qVar') st qnew l Delta (tl:UTTermList M.(terms) l) tl' v  *)
+(*   :  (forall xq, tau (ren xq) = sigma xq) *)
+(*      -> correctNaming tau v qnew *)
+(*      -> tl = SemTermList M tau tl' *)
+(*      -> SemTDec (M := M)(st := st) Delta tl v *)
+(*      -> Treelift M.(sortsI) (Pard atomI tau) (Pard SemNeg tau) (namedTypeTree tl' Delta qnew) v. *)
+
+(*   Proof. *)
+(*     move : l Delta tl tl'. *)
+(*     induction st => l Delta tl tl' H0 H1  H2; dependent induction v =>//=; dependent induction Delta =>//=; dependent induction qnew =>//=. *)
+(*     rewrite /getA/getTerms/ex2.  *)
+(*     by rewrite H2. *)
+(*     rewrite /getA/getTerms/ex2.  *)
+(*     by rewrite H2. *)
+(*     simpl in H1.  *)
+(*     elim: H1 => H3 H4. *)
+(*     move => [I1 I2]; split ; [apply (IHst1 _ _ _ _ tl) | apply (IHst2 _ _ _ _ tl) ] =>//. *)
+(*     simpl in H1.  *)
+(*     elim: H1 => H3 H4. *)
+(*     elim => H5 H6; split => //. *)
+(*     clear IHv IHDelta IHqnew. *)
+(*     apply (IHst _ _ _ _ (TermCons c Logic.I tl)) =>//. *)
+(*     simpl. *)
+(*     by rewrite SemTermsVar H3 H2. *)
+(* Qed. *)
+
+(*   Lemma compatrename w w' Gamma rho sigma tau (ren:w.(QVar) -> w'.(QVar)) *)
+(*   (pi: forall xq, tau (ren xq) = sigma xq) *)
+(*   : compat sigma Gamma rho -> compat tau (Contmap (w:=w) (fun i => i) (ParRen ren) (ParRen ren) Gamma) rho. *)
+(*   Proof. *)
+(*     rewrite/compat/Contlift/Contmap;elim => H1 [H2 H3] /=. *)
+(*                                               split => //;split. *)
+(*     move => xp. *)
+(*     move: (H2 xp); clear H2 H3. *)
+(*     elim : (readp Gamma xp) => l [a tl].  *)
+(*     rewrite /Pard/ParRen/ex1/getA/getTerms/ex2; simpl. *)
+(*     rewrite (SemTermListRen (QVar := w.(QVar)) (QVar' := w'.(QVar)) M ren sigma tau) =>//. *)
+(*     move => xn. *)
+(*     move: (H3 xn); clear H2 H3. *)
+(*     elim : (readn Gamma xn) => l [a tl].  *)
+(*     rewrite /Pard/ParRen/ex1/getA/getTerms/ex2; simpl. *)
+(*     rewrite (SemTermListRen (QVar := w.(QVar)) (QVar' := w'.(QVar)) M ren sigma tau) =>//. *)
+(* Qed. *)
+
+(* apply (SemPos2Treelift _ _ rho.(readq) _ (qinject Context (PatTree p) w) (PatTree p) (qnew Context (PatTree p) w) l Delta (SemTermList M rho.(readq) tl) (UTTermListRen (qinject Context (PatTree p) w) tl))=> // . *)
+(* move => xq. *)
+(* apply (Context.(extends_qinject) (w:=w) (st:=PatTree p)). *)
+(* apply (Context.(extends_qnew) (w:=w) (st:=PatTree p)). *)
+(* apply SemTermListRen. *)
+(* move => xq. *)
+(* apply (Context.(extends_qinject) (w:=w) (st:=PatTree p)). *)
+(* apply (compatrename _ _ _ _ rho.(readq)) => //. *)
+(* move => xq. *)
+(* apply (Context.(extends_qinject) (w:=w) (st:=PatTree p)). *)
