v3/Semantics.v
@@ -1,0 +1,661 @@
+Require Import ssreflect Basic SyntaxTyping List Coq.Program.Equality.
+
+(* We now define the semantics of terms according to a FullModelRaw *)
+Section TermSemantics.
+
+  (* A model has four support sets: terms, primitives, positives and negatives, and a
+relation ortho between negatives and positives *)
+  
+  Record Model4PTermsRaw := {
+                      terms      : Type;
+                      primitives : Type;
+                      positives  : Type;
+                      negatives  : Type;
+                      orth: negatives*positives -> Prop
+                    }
+  .
+
+  (* We first define semantical trees, which will interpret termtrees *)
+
+  Definition SemTree {M} := @Tree M.(terms) M.(primitives) M.(negatives).
+
+  (* This is a useful abbreviation for type valuations *)
+
+  Definition qvaluation {M} qVar := qVar -> M.(terms).
+
+  (* In order to build a model of proof-terms, we require an
+interpretation of terms, 
+an interpretation of patterns, 
+and an interpretation of the reifeied functions *)
+
+  Record Model4PTerms := 
+    {
+      model :> Model4PTermsRaw;
+
+      SemTerms {QVar}: @qvaluation model QVar -> Term QVar -> model.(terms);
+
+      SemTermsRen {QVar QVar'}:
+        forall (ren:QVar -> QVar') (sigma:@qvaluation model QVar) tau,
+          (forall xq, tau (ren xq) = sigma xq)
+          -> forall t, SemTerms sigma t = SemTerms tau (Term.(qrename) ren t);
+
+      SemTermsVar {QVar} sigma (xq:QVar): SemTerms sigma (Term.(varTerm) xq) = sigma xq;
+
+      tild : forall p:Patterns, @SemTree model (PatTree p) -> model.(positives);
+
+      I {w} : @ContType model.(terms) model.(primitives) model.(negatives) w
+              -> @Reifiable w
+              -> model.(negatives)
+    }.
+
+  Variable M: Model4PTerms.
+
+  Fixpoint SemTermList {qVar} sigma {P l} (tl:@TermList (Term qVar) P l)
+  :UTTermList M.(terms) l
+    := match tl with
+        | TermNil => TermNil
+        | TermCons r so H l' tl' => TermCons (M.(SemTerms) sigma r) Logic.I (SemTermList sigma tl')
+      end.
+
+  Lemma SemTermListRen {QVar QVar'}:
+        forall (ren:QVar -> QVar') (sigma:@qvaluation M QVar) tau,
+          (forall xq, tau (ren xq) = sigma xq)
+          -> forall l tl, SemTermList (l := l) sigma tl = SemTermList tau (UTTermListRen ren tl).
+  Proof.
+    intros.
+    induction l.
+    dependent inversion tl =>//.
+    dependent inversion tl =>//=.
+    rewrite (M.(SemTermsRen) (QVar := QVar) (QVar' := QVar') ren sigma tau) =>//.
+    by rewrite IHl.
+  Qed.
+
+  (* We apply our implementation of contexts to the notion of semantic
+contexts (aka valuations): positive (resp. negative) variables are
+mapped to positive (resp. negative) elements of the model *)
+  Definition SContext := @ContType M.(terms) M.(primitives) M.(negatives).
+
+  (* The semantics of a negative term is a negative element of the model *)
+  Definition SemN {w} (rho:SContext w) (tm : Neg) := 
+    match tm with
+      | rei f => M.(I) rho f
+    end
+  .
+
+  (* The semantics of a TermTree is a SemTree *)
+  Fixpoint SemSub {w} (rho:SContext w) {st} (v : TermTree st) {struct v} :=
+    match v in @TermTree _ s return SemTree s with
+      | tleafP xp => leafP (rho.(readp) xp)
+      | tleafN tm => leafN (SemN rho tm)
+      | tdummy    => dummy
+      | tnode s1 s2 v1 v2 => node (SemSub rho (st:=s1) v1) (SemSub rho (st:=s2) v2)
+      | tqnode s r v => qnode (M.(SemTerms) rho.(readq) r) (SemSub rho (st:=s) v)
+    end
+  .
+
+  (* The semantics of a positive term is a positive element of the model *)
+  Definition SemP {w} (rho:SContext w) (pt : Pos) := 
+    match pt with
+        pos p v => M.(tild) p (SemSub rho v)
+    end
+  .
+
+  (* The semantics of a command is a pair (negative element,positive
+element) of the model, that may or may not be orthogonal *) 
+
+  Definition SemC {w} (rho:SContext w) (c : Command) :=
+    match c with
+      | cut tm tp => (SemN rho tm,SemP rho tp) 
+      | select xm tp => (rho.(readn) xm,SemP rho tp)
+    end 
+  .
+
+  Definition SemOptionC {w} (rho:SContext w)(oc : OptionCommand) :=
+    match oc with
+      | some c => Some(SemC (rho:SContext w) c)
+      | none => None
+    end
+  .
+
+End TermSemantics.
+
+
+
+
+(************************************************************************)
+(* We now want to define the semantical interpretation of types/formulae.
+
+This is traditionally done "by induction on types/formulae".
+In our setting, we do not have an inductive structure for types/formulae;
+however, we know how to decompose molecules into atoms and
+molecules.
+
+Morally speaking, this corresponds to accessing sub-formulae, and
+since the sub-formula relation is the well-founded relation that
+allows to define the semantics of formulae, we will now assume the
+well-foundedness of the relation between molecules induced by the
+decomposition relation.
+
+In other words, when a molecule is decomposed into a TypeTree
+according to a pattern, then the molecules belonging to the TypeTree
+have to be SMALLER than the decomposed molecule.
+
+We formalise this. *)
+
+(* A molecule belongs to a TypeTree, as if it were a set *)
+
+Inductive  belong {l}
+: forall l' st, TypeTree st l' -> Molecule l -> Prop
+  :=
+  | rel_leaf  : forall B, belong l sleafN (TleafN B) B
+  | rel_node1 : forall B l' s1 s2 t1 t2,
+                  belong l' s1 t1 B -> belong l' (snode s1 s2) (Tnode t1 t2) B
+  | rel_node2 : forall B l' s1 s2 t1 t2,  
+                  belong l' s2 t2 B -> belong l' (snode s1 s2) (Tnode t1 t2) B
+  | rel_nodeq : forall so B l' s t, 
+                  belong (so::l') s t B
+                  -> belong l' (sqnode s) (Tqnode so t) B
+.
+
+Inductive relation : DPair Molecule -> DPair Molecule -> Prop :=
+  relation_base:
+    forall p l l' Delta A B, PatternsTyped p Delta A
+               -> belong l' (PatTree p) Delta B
+               -> relation (existS _ l B) (existS _ l' A).
+
+Hypothesis welf: well_founded relation.
+
+
+(****************************************************************)
+(* We now define the semantics of types according to a ModelRaw *)
+
+Section TypeSemantics.
+
+  Definition Pard {A B} {M:Model4PTerms} 
+             (f: forall a:DPair A, UTTermList (terms M) (ex1 a) -> B)
+             {qVar} sigma a
+    := f {{ ex1 a, getA (qVar := qVar) a }} (SemTermList M sigma (getTerms a)).
+  
+  Record ModelRaw :=
+    { model4PTerms :> Model4PTerms;
+      sortsI: Sorts -> model4PTerms.(terms) -> Prop;
+      sortscompat {qVar}: forall Sigma sigma,
+                            (forall qvar:qVar, sortsI (Sigma qvar) (sigma qvar))
+                            -> forall s t, 
+                                SortingRel Sigma t s
+                                -> sortsI s (model4PTerms.(SemTerms) sigma t);
+
+      atomI : forall a:DPair Atom,
+                UTTermList model4PTerms.(terms) (ex1 a)
+                -> model4PTerms.(primitives) -> Prop;
+
+      atomI_eq {qVar sigma}: forall a b p, is_eq a b
+                                  -> Pard (qVar := qVar) atomI sigma a p -> Pard atomI sigma b p
+
+    }.
+
+  Variable M: ModelRaw.
+
+  (* Here is the orthogonal of a set of positive elements of the model, or more precisely a predicate P: M.(positive) -> Prop *)
+  Definition ortho P :=
+    fun tm => forall tp: M.(positives), P tp -> M.(orth) (tm,tp).
+
+  (* Given a molecule A, this is a predicate on positives, that holds if
+this positive is of the form (M.(tild) p v), for some pattern p and
+some SemTree v such that p decomposes A into some TypeTree Delta and v is
+in the semantics of Delta. The semantics of TypeTrees not being defined
+yet, it is passed as an argument SemContext.  *)
+
+  Inductive PV
+            (A: DPair Molecule)
+            (SemContext: forall st, TypeTree st (ex1 A)
+                               -> forall tl:UTTermList M.(terms) (ex1 A), SemTree st -> Prop)
+            (tl: UTTermList M.(terms) (ex1 A))
+  : M.(positives) -> Prop :=
+    pv : forall p Delta v,
+           PatternsTyped p Delta (ex2 A)
+           -> SemContext (PatTree p) Delta tl v 
+           -> PV A SemContext tl (M.(tild) p v).
+
+  (* The interpretation (predicate on SemTrees) of a TypeTree Delta, given
+a valuation sigma and a function f that provides the negative
+interpretation of any molecule B in Delta *)
+
+  Definition SemCont_aux
+             (f : forall (A:DPair Molecule), UTTermList M.(terms) (ex1 A) -> M.(negatives) -> Prop)
+             l
+             st
+             (Delta : TypeTree st l)
+             (tl:UTTermList M.(terms) l)
+             (v: @SemTree M st)
+  : Prop.
+    move : l tl Delta.
+    induction st => l tl Delta; inversion Delta; inversion v.
+    exact (M.(atomI) {{ l, X }} tl X0).
+    exact (f {{ l, X }} tl X0).
+    exact True.
+    exact (IHst1 X1 l tl X /\ IHst2 X2 l tl X0).
+    exact ( M.(sortsI) so X0 /\ IHst X1 (so::l) (TermCons X0 (Logic.I) tl) X).
+  Defined.
+
+
+  (* The positive interpretation (predicate on positives) of a molecule
+A, given a valuation sigma that provides the positive interpretation of
+every molecule variable, and a function f that already provides the
+positive interpretation of any molecule B smaller than A *)
+
+  Definition SemPos_aux
+             (A: DPair Molecule)
+             (f : forall B, relation B A -> UTTermList M.(terms) (ex1 B) -> M.(positives) -> Prop)
+    := PV A (SemCont_aux (fun B tl tm => exists h:relation B A, ortho (f B h tl) tm) (ex1 A)).
+
+  (* The positive interpretation (predicate on positives) of a molecule
+A, given a type valuation sigma. Fixpoint of the previous function, built on
+the well-founded relation on molecules. *)
+
+  Definition SemPos := Fix welf _ (SemPos_aux).
+
+  (* The negative interpretation (predicate on negatives) of a molecule
+A, given a valuation sigma. It is built as the orthogonal of the positive
+interpretation of A.  *)
+
+  Definition SemNeg A tl := ortho (SemPos A tl).
+
+  (* A new version of the interpretation (predicate on SemTrees) of a
+TypeTree Delta, given a valuation sigma, but this time the predicate
+used as the negative interpretation of any molecule B in Delta is not
+passed as a parameter, it is the actual interpretation SemNeg *)
+
+  Definition SemCont {l st} := SemCont_aux SemNeg l st.
+
+  (* The definition of SemPos is so far quite cryptic, because of the
+induction that was necessary for the definition to be sound. The
+theorem below characterise SemPos in a much more intuitive way, but
+before that we need the following two lemmas. *)
+
+  Lemma F_ext_aux:
+    forall (x:DPair Molecule)
+      (f g: forall y:DPair Molecule, 
+              relation y x -> UTTermList M.(terms) (ex1 y) -> M.(positives) -> Prop),
+      (forall (y:DPair Molecule) (p:relation y x) tl d, f y p tl d <-> g y p tl d) 
+      -> forall st l (Delta:TypeTree st l),
+          forall tl' (v : SemTree st),
+            SemCont_aux (fun (B : DPair Molecule) tl (tm : negatives M) =>
+                           exists h : relation B x, ortho (f B h tl) tm)
+                        l st Delta tl' v ->
+            SemCont_aux (fun (B : DPair Molecule) tl (tm : negatives M) =>
+                           exists h : relation B x, ortho (g B h tl) tm)
+                        l st Delta tl' v .
+  Proof.
+    move => A f g H st.
+
+    induction st;
+      dependent induction v;
+      dependent induction Delta => //;simpl.
+
+    unfold ortho.
+    elim => h H1.
+    exists h.
+    move => tp H2.
+    apply: H1.
+    by apply H.
+
+    case => H1 H2.
+    by split; [apply: IHst1 |apply: IHst2].
+
+    clear  IHv.
+    move => [H1 H2].
+    split =>//.
+    by apply IHst.
+  Qed.
+
+  Lemma F_ext :
+    forall (x:DPair Molecule)
+      (f g: forall y:DPair Molecule, 
+              relation y x -> UTTermList M.(terms) (ex1 y) -> M.(positives) -> Prop),
+      (forall (y:DPair Molecule) (p:relation y x) tl d, f y p tl d <-> g y p tl d) 
+      -> forall tl d, SemPos_aux x f tl d -> SemPos_aux x g tl d.
+  Proof.
+    move => A f g H tl d.
+    unfold SemPos_aux.
+    elim.
+    intros.
+    apply (pv A _ tl p Delta v) => //.
+    move : v H1 ; clear H0 d.
+    apply F_ext_aux =>//. 
+  Qed.
+
+  Lemma Fix_F_inv :
+    forall (x:DPair Molecule) tl d (r s:Acc relation x),
+      Fix_F (fun A => UTTermList (terms M) (ex1 A) -> M.(positives) -> Prop) 
+            SemPos_aux r tl d 
+      <-> 
+      Fix_F (fun A => UTTermList (terms M) (ex1 A) -> M.(positives) -> Prop)
+            SemPos_aux s tl d.
+  Proof.
+    move => A; induction (welf A).
+    move => tl d r s.
+    rewrite <- (Fix_F_eq _ _ r). 
+    rewrite <- (Fix_F_eq _ _ s).
+    split.
+    apply (F_ext _
+                 (fun (y : DPair Molecule) (p : relation y x)  =>
+                    Fix_F _ SemPos_aux (Acc_inv r p))) => //=.
+    auto.
+    apply (F_ext _
+                 (fun (y : DPair Molecule) (p : relation y x)  =>
+                    Fix_F _ SemPos_aux (Acc_inv s p))) => //=.
+    auto.
+  Qed.
+
+  (* Characterisation of SemPos: The first step is to have a
+reformulation that looks much more like the definition of SemPos_aux,
+but with the actual SemPos taking the place of the parameter f *)
+
+  Lemma SemPos_Fix :
+    forall A tl tp, 
+      SemPos A tl tp 
+      <-> PV A 
+           (SemCont_aux (fun B tl' tm => exists h:relation B A, ortho (SemPos B tl') tm) (ex1 A))
+           tl
+           tp.
+  Proof.
+    move => A tl tp; unfold SemPos; unfold Fix in |- *.
+    rewrite <- Fix_F_eq.
+    split; apply F_ext; intros; apply Fix_F_inv.
+  Qed.
+
+  (* Characterisation of SemPos: The second step is to have a
+reformulation which drops the requirement B smaller than A in its use
+of SemCont_aux (that requirement was needed for the well-foundedness
+of the definition of SemPos) *)
+
+  Lemma SemPosCont_aux1 : 
+    forall A st l (Delta:TypeTree st l) tl (v:SemTree st), 
+      (forall B : DPair Molecule, belong l st Delta (ex2 B) -> relation B A)
+      -> SemCont_aux (fun (B : DPair Molecule) tl' (tm : negatives M) => 
+                       ortho (SemPos B tl') tm) 
+                    l st Delta tl v      
+      -> SemCont_aux (fun (B : DPair Molecule) tl' (tm : negatives M) =>
+                       exists _ : relation B A, ortho (SemPos B tl') tm)
+                    l st Delta tl v.
+  Proof.
+    move => A.
+    induction st;
+      dependent induction Delta ; move => tl v; 
+      dependent induction v => H //; simpl.
+
+      + move => H1.
+        assert (belong _ sleafN (TleafN m) m).
+        apply rel_leaf.
+        assert (relation (existS _ l m) A).
+        apply H => //=.
+        by exists H2.
+      + clear IHDelta1 IHDelta2 IHv1 IHv2.
+        elim => H3 H4.
+        split.
+        * apply IHst1 => //.
+          move => B H5.
+          apply: H.
+          apply: rel_node1 => //.
+        * apply: IHst2 => //.
+          move => B H5.
+          apply: H.
+          apply: rel_node2 => //.
+    + clear IHDelta IHv.
+        move => [H1 H2].
+        split =>//.
+        apply: IHst => //.
+        move => B H5.
+        apply: H.
+        apply: rel_nodeq => //.
+    Qed.
+
+  Lemma SemPosCont_aux2: 
+    forall A st l (Delta:TypeTree st l) tl (v:SemTree st), 
+      SemCont_aux (fun (B : DPair Molecule) tl' (tm : negatives M) =>
+                       exists _ : relation B A, ortho (SemPos B tl') tm)
+                    l st Delta tl v
+      -> SemCont_aux (fun (B : DPair Molecule) tl' (tm : negatives M) =>
+                       ortho (SemPos B tl') tm) 
+                    l st Delta tl v.
+  Proof.
+    move => A.
+    induction st;
+      dependent induction Delta ; move => tl v; 
+      dependent induction v => //; simpl.
+    + by move => [_ H] //=.
+    + by elim => H3 H4; split; [ apply IHst1 | apply IHst2].
+    + by move => [H4 H]; split => //; apply: IHst.
+    Qed.
+
+  Lemma SemPosCont_aux: 
+    forall A tl tp, 
+      PV A 
+         (SemCont_aux (fun B tl' tm => ortho (SemPos B tl') tm) (ex1 A))
+         tl
+         tp      
+      <-> PV A 
+           (SemCont_aux (fun B tl' tm => exists h:relation B A, ortho (SemPos B tl') tm) (ex1 A))
+           tl
+           tp.
+  Proof.
+    elim => lA Araw.
+    intros.
+    split => H;elim H;clear H;intros; apply (pv {{ lA,Araw }} _ tl p Delta v) => //=.
+    + assert  (forall (B : DPair Molecule),
+                 belong lA (PatTree p) Delta (ex2 B) -> relation B {{ lA,Araw }}).
+        * elim => lB Braw.
+          intros.
+          apply (relation_base p lB lA Delta) => //=.
+      apply SemPosCont_aux1 =>//.
+      apply (SemPosCont_aux2 {{ lA,Araw }}) =>//.
+  Qed.
+
+
+  (* Characterisation of SemPos: the final step is to write the
+definition we would actually like, and notice that, when unfolded, it
+is equivalent to the actual definition by using the previous two
+lemmas *)
+
+  Theorem SemPosCont : forall A tl tp, SemPos A tl tp <-> PV A (@SemCont (ex1 A)) tl tp.
+  Proof.
+    intros;split; intro.
+    apply SemPosCont_aux;apply SemPos_Fix => //=.
+    apply SemPos_Fix;apply SemPosCont_aux => //=.
+  Qed.
+
+End TypeSemantics.
+
+Arguments SemPos {M} _ _ _.
+Arguments SemCont {M} {l st} _ _ _.
+Arguments SemNeg {M} _ _ _.
+Arguments atomI {m} _ _ _.
+
+(**************************************)
+
+Section Adequacy.
+  
+  (* Even though we don't need to formalise a notion of reduction for
+proof-terms, the Adequacy Lemma requires from a model that its
+orthogonality relation be closed "under anti-reduction" *)
+
+  Record FullModel := 
+    {
+      M0 :> ModelRaw;
+
+      treevalue {st}: @SemTree M0 st -> Prop;
+
+      stab {w} :
+        forall (f: Reifiable) (rho: SContext M0 w) (p: Patterns) (v: SemTree (PatTree p)) c,
+          treevalue v
+          -> f p =cis= c
+          -> M0.(orth) (SemC M0 (Context.(extends) v rho) c)
+          -> M0.(orth) (M0.(I) rho f, M0.(tild) p v)
+    }.
+
+  Variable M:FullModel.
+
+  (* We define the interpretation of a typing context as a predicate on
+semantic contexts *)
+
+  Definition compat {w w'} val: @ContType Sorts 
+                                  (Par Atom w'.(QVar))
+                                  (Par Molecule w'.(QVar))
+                                  w
+                             -> SContext M w -> Prop
+    := Contlift (w := w) M.(sortsI)(Pard atomI val) (Pard SemNeg val).
+
+  Lemma SemPos2Treelift  qVar qVar' (sigma:qvaluation qVar) (tau:qvaluation qVar') (ren:qVar -> qVar') st qnew l Delta (tl:UTTermList M.(terms) l) tl' v 
+  :  (forall xq, tau (ren xq) = sigma xq)
+     -> correctNaming tau v qnew
+     -> tl = SemTermList M tau tl'
+     -> SemCont (M := M)(st := st) Delta tl v
+     -> Treelift M.(sortsI) (Pard atomI tau) (Pard SemNeg tau) (namedTypeTree tl' Delta qnew) v.
+
+  Proof.
+    move : l Delta tl tl'.
+    induction st => l Delta tl tl' H0 H1  H2; dependent induction v =>//=; dependent induction Delta =>//=; dependent induction qnew =>//=.
+    rewrite /getA/getTerms/ex2. 
+    by rewrite H2.
+    rewrite /getA/getTerms/ex2. 
+    by rewrite H2.
+    simpl in H1. 
+    elim: H1 => H3 H4.
+    move => [I1 I2]; split ; [apply (IHst1 _ _ _ _ tl) | apply (IHst2 _ _ _ _ tl) ] =>//.
+    simpl in H1. 
+    elim: H1 => H3 H4.
+    elim => H5 H6; split => //.
+    clear IHv IHDelta IHqnew.
+    apply (IHst _ _ _ _ (TermCons c Logic.I tl)) =>//.
+    simpl.
+    by rewrite SemTermsVar H3 H2.
+Qed.
+
+  Lemma compatrename w w' Gamma rho sigma tau (ren:w.(QVar) -> w'.(QVar))
+  (pi: forall xq, tau (ren xq) = sigma xq)
+  : compat sigma Gamma rho -> compat tau (Contmap (w:=w) (fun i => i) (ParRen ren) (ParRen ren) Gamma) rho.
+  Proof.
+    rewrite/compat/Contlift/Contmap;elim => H1 [H2 H3] /=.
+                                              split => //;split.
+    move => xp.
+    move: (H2 xp); clear H2 H3.
+    elim : (readp Gamma xp) => l [a tl]. 
+    rewrite /Pard/ParRen/ex1/getA/getTerms/ex2; simpl.
+    rewrite (SemTermListRen (QVar := w.(QVar)) (QVar' := w'.(QVar)) M ren sigma tau) =>//.
+    move => xn.
+    move: (H3 xn); clear H2 H3.
+    elim : (readn Gamma xn) => l [a tl]. 
+    rewrite /Pard/ParRen/ex1/getA/getTerms/ex2; simpl.
+    rewrite (SemTermListRen (QVar := w.(QVar)) (QVar' := w'.(QVar)) M ren sigma tau) =>//.
+Qed.
+
+  (* Here is finally the Adequacy Lemma *)
+
+  Hypothesis HValues: forall st (v:SemTree st) l Delta tl, SemCont (l := l) Delta tl v -> treevalue M v.
+
+  Theorem adequacy:
+    forall (w:World) (Gamma:TContext w),
+      (forall pt A,
+         TypingPos Gamma pt A
+         ->  forall rho, compat rho.(readq) Gamma rho
+                 -> Pard SemPos rho.(readq) A (SemP M rho pt)
+      )
+      /\ (forall l st (v:TermTree st) Delta tl,
+           TypingSub Gamma v Delta tl
+           ->  forall rho, compat rho.(readq) Gamma rho
+                   -> SemCont (l:=l) Delta (SemTermList M rho.(readq) tl) (SemSub M rho v)
+        )
+      /\ (forall nt A,
+           TypingNeg Gamma nt A
+           ->  forall rho, compat rho.(readq) Gamma rho
+                   -> Pard SemNeg rho.(readq) A (SemN M rho nt)
+        )
+      /\ (forall c,
+           TypingOptionCommand Gamma c
+           ->  forall rho, compat rho.(readq) Gamma rho
+                   -> exists csem, (SemOptionC M rho c) = Some csem /\ M.(orth) csem)
+      /\ (forall c,
+           TypingCommand Gamma c
+           ->  forall rho, compat rho.(readq) Gamma rho
+                   -> M.(orth) (SemC M rho c))
+  .
+    apply typing_ind;intros;
+    [
+      (* Typing a positive *)
+      apply SemPosCont; by apply (pv _ {{l, A}} _ _ p Delta) =>//; apply (H rho H0)
+
+      (* Typing a positive leaf of Sub *)
+      | unfold SemCont => //=;
+        by apply (M.(atomI_eq) (qVar:= w.(QVar)) (sigma:= rho.(readq)) 
+                        (Gamma.(readp) xp) {{l, (x, tl)}}) => //;
+        elim: H => _ [H _]; apply:H 
+
+      (* Typing a negative leaf of Sub *)
+      | unfold SemCont => //= ; by apply H
+
+      (* Typing a dummy leaf of Sub *)
+      | unfold SemCont => //= 
+
+      (* Typing a node of Sub *)
+      | by unfold SemCont => //=; unfold SemCont in H, H0; split; [apply H|apply H0]
+
+      (* Typing a qnode of Sub *)
+      | unfold SemCont => //=; 
+        by split;
+           [ apply (sortscompat M (Gamma.(readq))); move:H0;rewrite/compat/Contlift;elim => H2 _ 
+           | apply H ]
+
+      (* Typing a negative *)
+      | 
+
+      (* Typing an optional command *)
+      | by exists (SemC M rho c); split; [| apply: H]
+
+      (* Typing a cut *)
+      | by rewrite /SemCont/Pard/SemNeg/ortho/getA/getTerms in H;apply H =>//; apply H0
+
+      (* Typing a select *)
+      | by rewrite /SemC/compat/Pard/SemNeg/ortho in H0;apply H0;apply H
+    ].
+    
+    (* Typing a negative *)
+    rewrite /Pard/SemNeg/ortho/getA/getTerms => /= tp H1.
+    assert (PV M {{ l,A }} (@SemCont M l) (SemTermList M (readq rho) tl) tp)
+      by apply SemPosCont =>//=.
+    elim H2 => /= p Delta v H3 H4; clear H2.
+    have H6: (exists csem : negatives M * positives M,
+                SemOptionC (w:=Context.(wextends) (PatTree p) w)
+                           M
+                           (Context.(extends) v rho)
+                           (f p) = Some csem
+                /\ orth M csem).
+    apply: (H p Delta) => //.
+    apply (Context.(corr) (w:=w) (st:=PatTree p)).
+    apply (SemPos2Treelift _ _ rho.(readq) _ (qinject Context (PatTree p) w) (PatTree p) (qnew Context (PatTree p) w) l Delta (SemTermList M rho.(readq) tl) (UTTermListRen (qinject Context (PatTree p) w) tl))=> // .
+    move => xq.
+    apply (Context.(extends_qinject) (w:=w) (st:=PatTree p)).
+    apply (Context.(extends_qnew) (w:=w) (st:=PatTree p)).
+    apply SemTermListRen.
+    move => xq.
+    apply (Context.(extends_qinject) (w:=w) (st:=PatTree p)).
+    apply (compatrename _ _ _ _ rho.(readq)) => //.
+    move => xq.
+    apply (Context.(extends_qinject) (w:=w) (st:=PatTree p)).
+    elim: H6 => csem [H7 H8].
+    have : exists c, (f p = some c).
+    move : H7.
+    elim (f p) =>/=.
+    by move => c _; exists c.
+    move => H9;discriminate H9.
+    elim => c H9.
+    apply (M.(stab) (w:=w) _ _ _ _ c).
+    apply (HValues _ _ _ _ _ H4) =>//.
+    by rewrite H9.
+    move:H7.
+    rewrite H9 => /= H7; injection H7; clear H7 => H7; rewrite H7 =>//.
+  Qed.
+
+End Adequacy.
+
+Print Assumptions adequacy.
